Add sim_conf

src/localdrfra/PFtoRA.v
@@ -37,59 +37,157 @@ Require Import PFtoRAThread.
 Set Implicit Arguments.
 
 
+Definition option_rel3 {A B C} (P: A -> B -> C -> Prop)
+           (a: option A) (b: option B) (c: option C): Prop :=
+  match a, b, c with
+  | Some x, Some y, Some z => P x y z
+  | None, None, None => True
+  | _, _, _ => False
+  end.
+
+
 Module PFtoRA.
   Section PFtoRA.
     Variable L: Loc.t -> bool.
 
-    (* Definition option_rel3 {A B C} (P: A -> B -> C -> Prop) *)
-    (*            (a: option A) (b: option B) (c: option C): Prop := *)
-    (*   match a, b, c with *)
-    (*   | Some x, Some y, Some z => P x y z *)
-    (*   | None, None, None => True *)
-    (*   | _, _, _ => False *)
-    (*   end. *)
+    (* well-formedness *)
 
-    (* Inductive sim_thread_sl (tr: Trace.t) (views: Loc.t -> Time.t -> list View.t) (rels: ReleaseWrites.t) *)
-    (*           (sc_pf sc_j sc_ra: TimeMap.t) (mem_pf mem_j mem_ra: Memory.t): *)
-    (*   forall (sl_pf sl_j sl_ra: {lang: language & Language.state lang} * Local.t), Prop := *)
-    (* | sim_thread_sl_intro *)
-    (*     lang st_pf lc_pf st_j lc_j st_ra lc_ra *)
-    (*     (SIM: sim_thread L views rels *)
-    (*                      (Thread.mk lang st_pf lc_pf sc_pf mem_pf) *)
-    (*                      (Thread.mk lang st_j lc_j sc_j mem_j) *)
-    (*                      (Thread.mk lang st_ra lc_ra sc_ra mem_ra)) *)
-    (*     (SIM_TR: sim_trace tr rels) *)
-    (*     (TRACE_WF: TraceWF.wf tr lc_pf.(Local.promises) mem_pf) *)
-    (*     (RELS_WF: ReleaseWrites.wf rels lc_ra.(Local.promises) mem_ra): *)
-    (*     sim_thread_sl tr views rels sc_pf sc_j sc_ra mem_pf mem_j mem_ra *)
-    (*                   (existT _ lang st_pf, lc_pf) (existT _ lang st_j, lc_j) (existT _ lang st_ra, lc_ra) *)
-    (* . *)
+    Inductive wf_pf (tr: Trace.t) (c: Configuration.t): Prop :=
+    | wf_pf_intro
+        (WF: Configuration.wf c)
+        (TRACE: forall tid lang st lc
+                  (TH: IdentMap.find tid c.(Configuration.threads) = Some (existT _ lang st, lc)),
+            TraceWF.wf tr lc.(Local.promises) c.(Configuration.memory))
+    .
 
-    (* Inductive sim_conf (rels: ReleaseWrites.t): forall (c_pf c_ra: Configuration.t), Prop := *)
-    (* | sim_conf_intro *)
-    (*     views *)
-    (*     ths_pf sc_pf mem_pf *)
-    (*     ths_j sc_j mem_j *)
-    (*     ths_ra sc_ra mem_ra *)
-    (*     (THS: forall tid, *)
-    (*         option_rel3 *)
-    (*           (sim_thread_sl views rels sc_pf sc_j sc_ra mem_pf mem_j mem_ra) *)
-    (*           (IdentMap.find tid ths_pf) *)
-    (*           (IdentMap.find tid ths_j) *)
-    (*           (IdentMap.find tid ths_ra)): *)
-    (*     sim_conf rels *)
-    (*              (Configuration.mk ths_pf sc_pf mem_pf) *)
-    (*              (Configuration.mk ths_ra sc_ra mem_ra) *)
-    (* . *)
+    Definition wf_j := JConfiguration.wf.
 
-    (* Lemma sim_conf_steps *)
-    (*       views1 rels2 c1_pf c1_j c1_ra *)
-    (*       c2_pf trs *)
-    (*       (SIM: sim_conf views rels c1_pf c1_j c1_ra) *)
-    (*       (WF1_PF: Configuration.wf c1_pf) *)
-    (*       (WF1_J: Configuration.wf c1_j) *)
-    (*       (WF1_RA: Configuration.wf c1_ra) *)
-    (*       (STEPS_PF: LOCALDRF.configuration_steps_trace c1_pf c2_pf): *)
-    (*   exists  *)
+    Inductive wf_ra (rels: ReleaseWrites.t) (c: Configuration.t): Prop :=
+    | wf_ra_intro
+        (WF: Configuration.wf c)
+        (RELS: forall tid lang st lc
+                 (TH: IdentMap.find tid c.(Configuration.threads) = Some (existT _ lang st, lc)),
+            ReleaseWrites.wf rels lc.(Local.promises) c.(Configuration.memory))
+    .
+
+    Lemma wf_pf_thread
+          tr c tid lang st lc
+          (WF: wf_pf tr c)
+          (FIND: IdentMap.find tid c.(Configuration.threads) = Some (existT _ lang st, lc)):
+      PFtoRAThread.wf_pf tr (Thread.mk _ st lc c.(Configuration.sc) c.(Configuration.memory)).
+    Proof.
+      inv WF. inv WF0. inv WF.
+      hexploit THREADS; eauto. i.
+      hexploit TRACE; eauto. i.
+      econs; eauto.
+    Qed.
+
+    Lemma wf_j_thread
+          views c tid lang st lc
+          (WF: wf_j views c)
+          (FIND: IdentMap.find tid c.(Configuration.threads) = Some (existT _ lang st, lc)):
+      PFtoRAThread.wf_j views (Thread.mk _ st lc c.(Configuration.sc) c.(Configuration.memory)).
+    Proof.
+      inv WF. inv WF0. inv WF.
+      hexploit THREADS; eauto. i.
+      hexploit REL; eauto. i.
+      econs; eauto.
+    Qed.
+
+    Lemma wf_ra_thread
+          rels c tid lang st lc
+          (WF: wf_ra rels c)
+          (FIND: IdentMap.find tid c.(Configuration.threads) = Some (existT _ lang st, lc)):
+      PFtoRAThread.wf_ra rels (Thread.mk _ st lc c.(Configuration.sc) c.(Configuration.memory)).
+    Proof.
+      inv WF. inv WF0. inv WF.
+      hexploit THREADS; eauto. i.
+      hexploit RELS; eauto. i.
+      econs; eauto.
+    Qed.
+
+    Lemma step_wf_pf
+          tr1 tr e tid c1 c2
+          (WF1: wf_pf tr1 c1)
+          (STEP: pf_step_trace L tr e tid c1 c2):
+      <<WF2: wf_pf (tr1 ++ tr) c2>>.
+    Proof.
+      exploit pf_step_trace_future; eauto; try apply WF1. i. des.
+      inv STEP. ss.
+      exploit wf_pf_thread; eauto. i.
+      exploit Trace.steps_step_steps; eauto. i.
+      exploit PFtoRAThread.steps_pf_future; try exact x1; eauto. i. des.
+      econs; ss. i. Configuration.simplify; try apply x2.
+      exploit wf_pf_thread; try eapply TH; eauto. i. inv x3. ss.
+      apply TraceWF.wf_app.
+      - hexploit TraceWF.steps_disjoint_other; [eapply x0|eapply TRACE|..]; eauto.
+      - hexploit TraceWF.steps_disjoint; try eapply x1; eauto; try apply x0; s.
+        inv WF1. inv WF0. inv WF1. eauto.
+    Qed.
+
+    Lemma steps_wf_j
+          e tid c1 c2 views1 views2
+          (WF1: wf_j views1 c1)
+          (STEP: JConfiguration.step e tid c1 c2 views1 views2):
+      <<WF2: wf_j views2 c2>>.
+    Proof.
+      eapply JConfiguration.step_future; eauto.
+    Qed.
+
+    Lemma steps_wf_ra
+          e tid rels1 rels2 c1 c2
+          (WF1: wf_ra rels1 c1)
+          (STEP: RAConfiguration.step L e tid rels1 rels2 c1 c2):
+      <<WF2: wf_ra rels2 c2>>.
+    Proof.
+      exploit RAConfiguration.step_future; try eapply WF1; eauto. i. des.
+      inv STEP. ss.
+      assert (STEPS': RAThread.steps lang L rels1 rels2
+                                     (Thread.mk _ st1 lc1 c1.(Configuration.sc) c1.(Configuration.memory))
+                                     (Thread.mk _ st3 lc3 sc3 memory3)).
+      { exploit RAThread.tau_steps_steps; eauto. i.
+        inv STEP0; eapply RAThread.plus_step_steps; eauto. }
+      exploit wf_ra_thread; eauto. i.
+      hexploit RAThread.steps_rels_wf; try exact STEPS'; try apply x1. s. i.
+      econs; ss. i. Configuration.simplify; ss.
+      exploit wf_ra_thread; try eapply TH; eauto. i.
+      inv WF1. inv WF. inv WF0.
+      exploit DISJOINT; try exact n; eauto. i.
+      hexploit RAThread.steps_rels_disjoint; try exact x; eauto. apply x1.
+    Qed.
+
+
+    (* sim *)
+
+    Inductive sim_thread_sl (views: Loc.t -> Time.t -> list View.t) (rels: ReleaseWrites.t)
+              (sc_pf sc_j sc_ra: TimeMap.t) (mem_pf mem_j mem_ra: Memory.t):
+      forall (sl_pf sl_j sl_ra: {lang: language & Language.state lang} * Local.t), Prop :=
+    | sim_thread_sl_intro
+        lang st_pf lc_pf st_j lc_j st_ra lc_ra
+        (SIM: PFtoRAThread.sim_thread L views rels
+                                      (Thread.mk lang st_pf lc_pf sc_pf mem_pf)
+                                      (Thread.mk lang st_j lc_j sc_j mem_j)
+                                      (Thread.mk lang st_ra lc_ra sc_ra mem_ra)):
+        sim_thread_sl views rels sc_pf sc_j sc_ra mem_pf mem_j mem_ra
+                      (existT _ lang st_pf, lc_pf) (existT _ lang st_j, lc_j) (existT _ lang st_ra, lc_ra)
+    .
+
+    Inductive sim_conf (tr: Trace.t) (rels: ReleaseWrites.t): forall (c_pf c_ra: Configuration.t), Prop :=
+    | sim_conf_intro
+        views
+        ths_pf sc_pf mem_pf
+        ths_j sc_j mem_j
+        ths_ra sc_ra mem_ra
+        (SIM_TR: PFtoRAThread.sim_trace tr rels)
+        (THS: forall tid,
+            option_rel3
+              (sim_thread_sl views rels sc_pf sc_j sc_ra mem_pf mem_j mem_ra)
+              (IdentMap.find tid ths_pf)
+              (IdentMap.find tid ths_j)
+              (IdentMap.find tid ths_ra)):
+        sim_conf tr rels
+                 (Configuration.mk ths_pf sc_pf mem_pf)
+                 (Configuration.mk ths_ra sc_ra mem_ra)
+    .
   End PFtoRA.
 End PFtoRA.
